feat(lts): step instances of choice/countable

theories/concur/lts.v
@@ -197,11 +197,14 @@ End Def.
 
 Prenex Implicits lbl src dst is_step step_of adj.
 
-Section EQ. 
-Context {L : eqType} (S : ltsType L).
+Section Prod. 
+Context {L : Type} (S : ltsType L).
 
 Definition prod_of_step : stepTuple S -> L * S * S := 
   fun s => (lbl s, src s, dst s).
+
+Definition step_of_prod : L * S * S -> option (step S) := 
+  fun '(lbl, src, dst) => insub (mk_step lbl src dst).
 
 Lemma prod_of_step_inj : injective prod_of_step.
 Proof. 
@@ -209,17 +212,44 @@ Proof.
   by case x; case y=> /= ?????? -> -> ->. 
 Qed.
 
-Definition stepTuple_eqMixin := InjEqMixin prod_of_step_inj.
+Lemma prod_of_stepK : 
+  pcancel (prod_of_step : step S -> L * S * S) step_of_prod.
+Proof. 
+  move=> st /=; rewrite insubT=> /=.
+  - by move: (valP st); rewrite /is_step.
+  move=> H /=; congr Some; apply/val_inj=> /=. 
+  by move: H=> _; case: st=> [[]] /=.  
+Qed.
+
+End Prod.
+
+Section EQ.
+Context {L : eqType} (S : ltsType L).
+
+Definition stepTuple_eqMixin := InjEqMixin (@prod_of_step_inj L S).
 Canonical stepTuple_eqType := 
   Eval hnf in EqType (stepTuple S) stepTuple_eqMixin.
 
 Definition step_eqMixin := Eval hnf in [eqMixin of step S by <:].
 Canonical step_eqType := Eval hnf in EqType (step S) step_eqMixin.
 
-(* Variables (st1 st2 : step S). *)
-(* Check (st1 == st2). *)
-
 End EQ.
+
+Section Choice.
+Context {L : choiceType} (S : ltsType L).
+
+Definition step_choiceMixin := PcanChoiceMixin (@prod_of_stepK L S).
+Canonical step_choiceType := Eval hnf in ChoiceType (step S) step_choiceMixin.
+
+End Choice.
+
+Section Countable.
+Context {L : countType} (S : ltsType L).
+
+Definition step_countMixin := PcanCountMixin (@prod_of_stepK L S).
+Canonical step_countType := Eval hnf in CountType (step S) step_countMixin.
+
+End Countable.
 
 Section Theory.
 Context {L : eqType} (S : ltsType L).
